theories/L/Complexity/Cook/PTPR_Preludes.v
@@ -23,6 +23,24 @@ Require Import Lia.
   that preludes allow one to reduce an existential question to another (possibly simpler) existential question.
   *)
 
+Section defExPTPR. 
+  (*original instance lacking an initial string*)
+  Variable (Sigma : finType). 
+
+  (*we do not directly assume Sigma to be a finType in order to be able to use the definitions not depending on Sigma being a finType for ordinary Types *)
+
+  Variable (p : Sigma -> Sigma -> Sigma -> Sigma -> Sigma -> Sigma -> Prop). 
+  Variable (finalCondition : list (list Sigma)). 
+  Variable (t : nat). 
+
+  (*instead of an initial string, we have an initial condition and a length l*)
+  Variable (initCond: list Sigma -> Prop). 
+  Variable (l : nat).
+
+  (*the question now is: does there exist x0 satisfying initCond such that it ends up in a final state? *)
+  Definition ExPTPR := exists x0, |x0| = l /\ initCond x0 /\ PTPRLang (Build_PTPR x0 p finalCondition t). 
+End defExPTPR.
+
 Section fixPTPRInstance. 
   (*original instance lacking an initial string*)
   Variable (Sigma : Type). 
@@ -35,15 +53,11 @@ Section fixPTPRInstance.
   Variable (finalCondition : list (list Sigma)). 
   Variable (t : nat). 
 
-  (*instead of an initial string, we have an initial condition and a length l*)
   Variable (initCond: list Sigma -> Prop). 
   Variable (l : nat).
 
   (*otherwise, vacuous rewrites destroy everything *)
   Variable (A0 : l >= 3). 
-
-  (*the question now is: does there exist x0 satisfying initCond such that it ends up in a final state? *)
-  Definition ExPTPR := exists x0, |x0| = l /\ initCond x0 /\ PTPRLang (Build_PTPR x0 p finalCondition t). 
 
   (*a prelude generates initial strings satisfying initCond *)
   Variable (Sigma' : Type). 
@@ -52,7 +66,10 @@ Section fixPTPRInstance.
 
   Notation combSigma := (sum Sigma Sigma').
   Variable (p' : Sigma' -> Sigma' -> Sigma' -> combSigma -> combSigma -> combSigma -> Prop). 
-  Variable (initialString : list Sigma').   
+  (*We prove the following results not for a fixed initial string, but for a string satisfying initialPred.
+    This allows us to compose multiple preludes, each reducing to a simpler ExPTPR instance.
+  *)
+  Variable (initialPred : list Sigma' -> Prop).   
   Variable (t' : nat). 
 
   Definition isOrigString (s : list combSigma) := exists s', s = map inl s'.  
@@ -69,20 +86,19 @@ Section fixPTPRInstance.
   Definition combP a b c d e f := liftPrelude a b c d e f \/ liftOrig a b c d e f.
   Hint Unfold combP. 
 
+  Definition validPreludeInitial s := length s = l /\ initialPred s. 
+
   (*the prelude rules always produce a string that is a valid initial string for the original instance, up to the injection inl *)
-  Variable (A1: forall x0, relpower (valid (rewritesHeadInd liftPrelude)) t' (map inr initialString) x0 -> isOrigString x0). 
+  Variable (A1: forall init x0, validPreludeInitial init -> relpower (valid (rewritesHeadInd liftPrelude)) t' (map inr init) x0 -> isOrigString x0). 
 
   (*disjointness: string is not produced too early *)
-  Variable (A2 : forall k x, k < t' -> relpower (valid (rewritesHeadInd liftPrelude)) k (map inr initialString) x -> isPreludeString x).  
+  Variable (A2 : forall init k x, validPreludeInitial init -> k < t' -> relpower (valid (rewritesHeadInd liftPrelude)) k (map inr init) x -> isPreludeString x).  
 
   (*completeness *)
-  Variable (A3 : forall x0, initCond x0 /\ |x0| = l -> relpower (valid (rewritesHeadInd liftPrelude)) t' (map inr initialString) (map inl x0)). 
+  Variable (A3 : forall x0, initCond x0 /\ |x0| = l -> exists init, validPreludeInitial init /\ relpower (valid (rewritesHeadInd liftPrelude)) t' (map inr init) (map inl x0)). 
 
   (*soundness *)
-  Variable (A4 : forall x0, relpower (valid (rewritesHeadInd liftPrelude)) t' (map inr initialString) x0 -> exists x0', x0 = map inl x0' /\ initCond x0'). 
-
-  (*compatibility *)
-  Variable (A5 : |initialString| = l). 
+  Variable (A4 : forall init x0, validPreludeInitial init -> relpower (valid (rewritesHeadInd liftPrelude)) t' (map inr init) x0 -> exists x0', x0 = map inl x0' /\ initCond x0'). 
 
   Lemma liftPrelude_subs_combP : windowPred_subs liftPrelude combP. 
   Proof. 
@@ -96,114 +112,112 @@ Section fixPTPRInstance.
     | [H : [] = map _ ?s |- _] => is_var s; destruct s; cbn in H; [ clear H| congruence]
   end. 
 
-  Lemma relpower_inr_liftPrelude' n b: 
-    n < t' 
-    -> relpower (valid (rewritesHeadInd combP)) n (map inr initialString) b 
-    -> relpower (valid (rewritesHeadInd liftPrelude)) n (map inr initialString) b /\ isPreludeString b.
-  Proof. 
-    intros H0 H. clear A0 A1 A3 A4 A5. 
-    remember (map inr initialString). 
-    (*we use the version of relpower defined by adding transitions at the tail of a chain since we need to keep A2, which requires the initialString at the head (otherwise, we could not apply the IH) *)
-    apply relpower_relpowerRev in H. setoid_rewrite relpower_relpowerRev. 
-    induction H; cbn; intros; subst. 
-    - eauto. 
-    - edestruct (IHrelpowerRev) as (IH & (? & ->)). 
-      + reflexivity. 
-      + apply A2. 
-      + lia. 
-      + clear IHrelpowerRev. assert (valid (rewritesHeadInd liftPrelude) (map inr x) y') as H3.   
+  Section fixInitial.
+    Variable (initialString : list Sigma').
+    Context {Hinitial : validPreludeInitial initialString}.
+
+    Lemma relpower_inr_liftPrelude' n b: 
+      n < t' 
+      -> relpower (valid (rewritesHeadInd combP)) n (map inr initialString) b 
+      -> relpower (valid (rewritesHeadInd liftPrelude)) n (map inr initialString) b /\ isPreludeString b.
+    Proof. 
+      intros H0 H. clear A0 A1 A3 A4. 
+      remember (map inr initialString). 
+      (*we use the version of relpower defined by adding transitions at the tail of a chain since we need to keep A2, which requires the initialString at the head (otherwise, we could not apply the IH) *)
+      apply relpower_relpowerRev in H. setoid_rewrite relpower_relpowerRev. 
+      induction H; cbn; intros; subst. 
+      - eauto. 
+      - edestruct (IHrelpowerRev) as (IH & (? & ->)). 
+        + lia. 
+        + reflexivity. 
+        + clear IHrelpowerRev. assert (valid (rewritesHeadInd liftPrelude) (map inr x) y') as H3.   
+          { 
+            clear IH H0 H. remember (map inr x) as x' eqn:H2. revert x H2. 
+            induction H1; cbn; intros; eauto; inv_eqn_map. 
+            + constructor 2; [eapply IHvalid; reflexivity | apply H]. 
+            + constructor 3; [eapply IHvalid; reflexivity | clear IHvalid]. 
+              inv H. inv_eqn_map.
+              inv H2;  [eauto |  ]. inv H. 
+          } 
+          split. 
+          * apply relpowerRevS with (y := map inr x); [ apply IH | apply H3]. 
+          * (*we use A2 to derive that b is a preludeString *)
+            assert (relpower (valid (rewritesHeadInd liftPrelude)) (S n) (map inr initialString) y') as H2. 
+            { apply relpower_relpowerRev. eauto. }
+            now apply A2 in H2. 
+    Qed.  
+
+    Corollary relpower_inr_liftPrelude n b : 
+      n <= t' 
+      -> relpower (valid (rewritesHeadInd combP)) n (map inr initialString) b 
+      -> relpower (valid (rewritesHeadInd liftPrelude)) n (map inr initialString) b.
+    Proof. 
+      intros. clear A0 A1 A3 A4. destruct (lt_dec n t') as [l0 | l0]. 
+      - eapply relpower_inr_liftPrelude' in H0; [ | apply l0]. tauto. 
+      - assert (n = t') by lia. clear H l0. destruct n. 
+        + inv H0. auto. 
+        + assert (n < t') as H2 by lia. apply relpower_relpowerRev in H0. inversion H0. 
+          apply relpower_relpowerRev in H3. apply relpower_inr_liftPrelude' in H3 as (H3 & (? & ->)); subst; [ | apply H2].
+          apply relpower_relpowerRev. econstructor; [ apply relpower_relpowerRev, H3 | ]. 
+          clear H2 H3 H0 A2. remember (map inr x0) as x1 eqn:Heqn. revert x0 Heqn. induction H4; intros.  
+          * eauto. 
+          * inv_eqn_map; constructor; eauto.
+          * inv_eqn_map; constructor 3; [eauto | ]. inv H. inv_eqn_map. inv H1; [ eauto | ]. inv H. 
+    Qed. 
+
+    Lemma relpower_inl_liftOrig n s b : 
+      |s| >= 3  
+      -> relpower (valid (rewritesHeadInd combP)) n (map inl s) b 
+      -> relpower (valid (rewritesHeadInd liftOrig)) n (map inl s) b /\ isOrigString b. 
+    Proof. 
+      clear A0 A1 A2 A3 A4. intros H0 H. remember (map inl s) as s' eqn:Heqn. 
+      enough (relpower (valid (rewritesHeadInd liftOrig)) n s' b /\ isOrigString b) by tauto. 
+      revert s H0 Heqn. 
+      induction H; intros.  
+      - subst; split; unfold isOrigString; eauto. 
+      - assert (valid (rewritesHeadInd liftOrig) a b /\ isOrigString b) as (H2 & (? & ->)). 
         { 
-          clear IH H0 H. remember (map inr x) as x' eqn:H2. revert x H2. 
-          induction H1; cbn; intros; eauto; inv_eqn_map. 
-          + constructor 2; [eapply IHvalid; reflexivity | apply H]. 
-          + constructor 3; [eapply IHvalid; reflexivity | clear IHvalid]. 
-            inv H. inv_eqn_map.
-            inv H2;  [eauto |  ]. inv H. 
+          clear IHrelpower H0. revert s H1 Heqn. unfold isOrigString. induction H; intros. 
+          + eauto. 
+          + inv_eqn_map. rewrite map_length in H0; cbn in H1; lia.   
+          + inv_eqn_map. inv H0. inv_eqn_map. inv H3. 
+            * inv H0.   
+            * inv H0. destruct s4; cbn in *. 
+              -- apply valid_length_inv in H; destruct s2; [ | cbn in H; congruence]. 
+                 split.
+                 ++ constructor 3. constructor 2; cbn; eauto.  eauto.
+                 ++ exists [d; e; f]; eauto. 
+              -- edestruct (IHvalid (s0::s3::s1::s4)) as (H2 & (? & H3)); [now cbn | now cbn | inv_eqn_map ]. 
+                 split; [eauto | ]. exists (d :: s5 :: s6 :: x); eauto.  
         } 
-        split. 
-        * apply relpowerRevS with (y := map inr x); [ apply IH | apply H3]. 
-        * (*we use A2 to derive that b is a preludeString *)
-          assert (relpower (valid (rewritesHeadInd liftPrelude)) (S n) (map inr initialString) y') as H2. 
-          { apply relpower_relpowerRev. eauto. }
-          now apply A2 in H2. 
-  Qed.  
+        subst. 
+        edestruct (IHrelpower) as (IH1 & IH2). 
+        2: { reflexivity. }
+        + apply valid_length_inv in H. rewrite !map_length in H. lia. 
+        + split; [ | apply IH2]. apply relpowerS with (b := map inl x); [ apply H2 |apply IH1].  
+    Qed. 
 
-  Corollary relpower_inr_liftPrelude n b : 
-    n <= t' 
-    -> relpower (valid (rewritesHeadInd combP)) n (map inr initialString) b 
-    -> relpower (valid (rewritesHeadInd liftPrelude)) n (map inr initialString) b.
-  Proof. 
-    intros. clear A0 A1 A3 A4 A5. destruct (lt_dec n t') as [l0 | l0]. 
-    - eapply relpower_inr_liftPrelude' in H0; [ | apply l0]. tauto. 
-    - assert (n = t') by lia. clear H l0. destruct n. 
-      + inv H0. auto. 
-      + assert (n < t') as H2 by lia. apply relpower_relpowerRev in H0. inversion H0. 
-        apply relpower_relpowerRev in H3. apply relpower_inr_liftPrelude' in H3 as (H3 & (? & ->)); subst; [ | apply H2].
-        apply relpower_relpowerRev. econstructor; [ apply relpower_relpowerRev, H3 | ]. 
-        clear H2 H3 H0 A2. remember (map inr x0) as x1 eqn:Heqn. revert x0 Heqn. induction H4; intros.  
-        * eauto. 
-        * inv_eqn_map; constructor; eauto.
-        * inv_eqn_map; constructor 3; [eauto | ]. inv H. inv_eqn_map. inv H1; [ eauto | ]. inv H. 
-  Qed. 
+    (*important intermediate result for the proof: we can split a sequence of t' + t rewrite steps into t' rewrite steps of the prelude and t rewrite steps of the original PR instance *)
+    Lemma relpower_comb_split sf : 
+      relpower (valid (rewritesHeadInd combP)) (t' + t) (map inr initialString) sf 
+      -> exists x0, relpower (valid (rewritesHeadInd liftPrelude)) t' (map inr initialString) x0 
+                    /\ relpower (valid (rewritesHeadInd liftOrig)) t x0 sf /\ isOrigString sf.
+    Proof. 
+      clear A3 A4. 
+      intros (z & H1 & H2)%relpower_add_split. 
+      exists z. apply relpower_inr_liftPrelude in H1; [ | auto]. split. 
+      - eauto. 
+      - specialize (A1 Hinitial H1) as (? & ->). eapply relpower_inl_liftOrig. 
+        + clear H2 A2. 
+          apply relpower_valid_length_inv in H1. rewrite !map_length in H1. rewrite <-H1, (proj1 Hinitial). lia. 
+        + apply H2. 
+    Qed. 
+  End fixInitial. 
 
-  Lemma relpower_add_split (X : Type) (R : X -> X -> Prop) n m x y: relpower R (n + m) x y -> exists z, relpower R n x z /\ relpower R m z y.
-  Proof. 
-    clear A0 A1 A2 A3 A4 A5. 
-    revert x y. induction n; intros. 
-    - cbn in H. eauto. 
-    - inv H. apply IHn in H2 as (z & H3 & H4). exists z. eauto.
-  Qed. 
-
-  Lemma relpower_inl_liftOrig n s b : 
-    |s| >= 3  
-    -> relpower (valid (rewritesHeadInd combP)) n (map inl s) b 
-    -> relpower (valid (rewritesHeadInd liftOrig)) n (map inl s) b /\ isOrigString b. 
-  Proof. 
-    clear A0 A1 A2 A3 A4 A5. intros H0 H. remember (map inl s) as s' eqn:Heqn. 
-    enough (relpower (valid (rewritesHeadInd liftOrig)) n s' b /\ isOrigString b) by tauto. 
-    revert s H0 Heqn. 
-    induction H; intros.  
-    - subst; split; unfold isOrigString; eauto. 
-    - assert (valid (rewritesHeadInd liftOrig) a b /\ isOrigString b) as (H2 & (? & ->)). 
-      { 
-        clear IHrelpower H0. revert s H1 Heqn. unfold isOrigString. induction H; intros. 
-        + eauto. 
-        + inv_eqn_map. rewrite map_length in H0; cbn in H1; lia.   
-        + inv_eqn_map. inv H0. inv_eqn_map. inv H3. 
-          * inv H0.   
-          * inv H0. destruct s4; cbn in *. 
-            -- apply valid_length_inv in H; destruct s2; [ | cbn in H; congruence]. 
-               split.
-               ++ constructor 3. constructor 2; cbn; eauto.  eauto.
-               ++ exists [d; e; f]; eauto. 
-            -- edestruct (IHvalid (s0::s3::s1::s4)) as (H2 & (? & H3)); [now cbn | now cbn | inv_eqn_map ]. 
-               split; [eauto | ]. exists (d :: s5 :: s6 :: x); eauto.  
-      } 
-      subst. 
-      edestruct (IHrelpower) as (IH1 & IH2). 
-      2: { reflexivity. }
-      + apply valid_length_inv in H. rewrite !map_length in H. lia. 
-      + split; [ | apply IH2]. apply relpowerS with (b := map inl x); [ apply H2 |apply IH1].  
-  Qed. 
-
-  Lemma relpower_comb_split sf : 
-    relpower (valid (rewritesHeadInd combP)) (t' + t) (map inr initialString) sf 
-    -> exists x0, relpower (valid (rewritesHeadInd liftPrelude)) t' (map inr initialString) x0 
-                  /\ relpower (valid (rewritesHeadInd liftOrig)) t x0 sf /\ isOrigString sf.
-  Proof. 
-    clear A3 A4. 
-    intros (z & H1 & H2)%relpower_add_split. 
-    exists z. apply relpower_inr_liftPrelude in H1; [ | auto]. split. 
-    - eauto. 
-    - specialize (A1 H1) as (? & ->). eapply relpower_inl_liftOrig. 
-      + clear H2 A2. 
-        apply relpower_valid_length_inv in H1. rewrite !map_length in H1. lia. 
-      + apply H2. 
-  Qed. 
-
+  (*we need to be able to go back from liftOrig to p*)
   Lemma valid_liftOrig_isOrigString a b : |a| >= 3 -> valid (rewritesHeadInd liftOrig) a b -> isOrigString b. 
   Proof. 
-    clear A1 A2 A3 A4 A5 A0. intros H. induction 1; unfold isOrigString. 
+    clear A1 A2 A3 A4 A0. intros H. induction 1; unfold isOrigString. 
     - exists []; eauto.
     - cbn in H; lia. 
     - cbn in H. inv H1. destruct s1. 
@@ -215,7 +229,7 @@ Section fixPTPRInstance.
 
   Lemma liftOrig_valid_p x x': valid (rewritesHeadInd liftOrig) (map inl x) (map inl x') -> valid (rewritesHeadInd p) x x'.
   Proof. 
-    clear A1 A2 A3 A4 A5 A0. 
+    clear A1 A2 A3 A4 A0. 
     remember (map inl x) as x0 eqn:eqnx0. remember (map inl x') as x0' eqn:eqnx0'. 
     induction 1 in x, x', eqnx0, eqnx0' |- *; inv_eqn_map. 
     - eauto. 
@@ -230,7 +244,7 @@ Section fixPTPRInstance.
     -> relpower (valid (rewritesHeadInd liftOrig)) n (map inl x) (map inl sf) 
     -> relpower (valid (rewritesHeadInd p)) n x sf. 
   Proof. 
-    clear A1 A2 A3 A4 A5 A0. intros H0 H. remember (map inl x) as x' eqn:Hx'. remember (map inl sf) as sf' eqn:Hsf'. 
+    clear A1 A2 A3 A4 A0. intros H0 H. remember (map inl x) as x' eqn:Hx'. remember (map inl sf) as sf' eqn:Hsf'. 
     revert x sf H0 Hx' Hsf'. induction H; intros. 
     - subst; apply Prelim.map_inj in Hsf'; [ subst; auto| unfold injective; intros; congruence]. 
     - assert (|a| >= 3). { subst. rewrite map_length. apply H1. } 
@@ -240,7 +254,91 @@ Section fixPTPRInstance.
         subst. apply valid_length_inv in H. now rewrite !map_length in H.  
   Qed. 
 
-  Lemma prelude_ok : ExPTPR <-> PTPRLang (Build_PTPR (map inr initialString) combP (map (map inl) finalCondition) (t' + t)). 
+  (*TODO: reduction to ExPTPR *)
+End fixPTPRInstance.
+
+(*we now specialise to the case where the initial condition on the prelude string is fixed to equality with a given string, 
+  i.e. we reduce an ExPTPR instance to a full PTPR instance
+*)
+Section fixPrelude. 
+  Variable (Sigma : Type). 
+
+  (*we do not directly assume Sigma to be a finType in order to be able to use the definitions not depending on Sigma being a finType for ordinary Types *)
+  Variable (ESigma : eq_dec Sigma). 
+  Variable (FSigma : finTypeC (EqType Sigma)). 
+
+  Variable (p : Sigma -> Sigma -> Sigma -> Sigma -> Sigma -> Sigma -> Prop). 
+  Variable (finalCondition : list (list Sigma)). 
+  Variable (t : nat). 
+
+  Variable (initCond: list Sigma -> Prop). 
+  Variable (l : nat).
+
+  (*otherwise, vacuous rewrites destroy everything *)
+  Variable (A0 : l >= 3). 
+
+  (*a prelude generates initial strings satisfying initCond *)
+  Variable (Sigma' : Type). 
+  Variable (eSigma' : eq_dec Sigma').
+  Variable (FSigma' : finTypeC (EqType Sigma')). 
+
+  Notation combSigma := (sum Sigma Sigma').
+  Variable (p' : Sigma' -> Sigma' -> Sigma' -> combSigma -> combSigma -> combSigma -> Prop). 
+
+  (*we now specialise to a fixed initial string *)
+  Variable (initialString : list Sigma').
+  Variable (t' : nat). 
+
+  Hint Constructors liftPrelude liftOrig.
+  Hint Unfold combP. 
+
+  Notation liftPrelude := (liftPrelude p').
+  Notation combP := (combP p p').
+
+  (*the prelude rules always produce a string that is a valid initial string for the original instance, up to the injection inl *)
+  Variable (A1: forall x0, relpower (valid (rewritesHeadInd liftPrelude)) t' (map inr initialString) x0 -> isOrigString x0). 
+
+  (*disjointness: string is not produced too early *)
+  Variable (A2 : forall k x, k < t' -> relpower (valid (rewritesHeadInd liftPrelude)) k (map inr initialString) x -> isPreludeString x).  
+
+  (*completeness *)
+  Variable (A3 : forall x0, initCond x0 /\ |x0| = l -> relpower (valid (rewritesHeadInd liftPrelude)) t' (map inr initialString) (map inl x0)). 
+
+  (*soundness *)
+  Variable (A4 : forall x0, relpower (valid (rewritesHeadInd liftPrelude)) t' (map inr initialString) x0 -> exists x0', x0 = map inl x0' /\ initCond x0'). 
+
+  Variable (A5 : length initialString = l). 
+
+  (*We use the results of the previous section. For that, we setup the initial condition and prove the assumptions the previous section has. *)
+  Definition preludeInitialPred s := s = initialString. 
+
+  Notation validPreludeInitial := (validPreludeInitial l preludeInitialPred). 
+
+  Fact A1p init x0 : validPreludeInitial init -> relpower (valid (rewritesHeadInd liftPrelude)) t' (map inr init) x0 -> isOrigString x0.
+  Proof. 
+    intros [H1 ->]. easy.
+  Qed. 
+
+  Fact A2p init k x: validPreludeInitial init -> k < t' -> relpower (valid (rewritesHeadInd liftPrelude)) k (map inr init) x -> isPreludeString x.
+  Proof. 
+    intros [H1 ->]. easy. 
+  Qed. 
+
+  Fact A3p x0: initCond x0 /\ |x0| = l -> exists init, validPreludeInitial init /\ relpower (valid (rewritesHeadInd liftPrelude)) t' (map inr init) (map inl x0).
+  Proof. 
+    intros [H1 H2]. exists initialString. split; [ | easy]. split; [easy | reflexivity]. 
+  Qed. 
+
+  Fact A4p init x0: validPreludeInitial init -> relpower (valid (rewritesHeadInd liftPrelude)) t' (map inr init) x0 -> exists x0', x0 = map inl x0' /\ initCond x0'.
+  Proof. 
+    intros [H1 ->]. easy. 
+  Qed. 
+
+  Fact initialString_validPreludeInitial : validPreludeInitial initialString. 
+  Proof. easy. Qed. 
+
+  (*the main result *)
+  Lemma prelude_ok : ExPTPR p finalCondition t initCond l <-> PTPRLang (Build_PTPR (map inr initialString) combP (map (map inl) finalCondition) (t' + t)). 
   Proof. 
     split. 
     - intros (x0 & H1 & H2 & (_ & sf & F1 & F2)). cbn in *. split. 
@@ -265,10 +363,10 @@ Section fixPTPRInstance.
           exists (map inl b1), (map inl b2). now rewrite F3, !map_app. 
     - intros (_ & sf & F1 & F2). cbn in *. unfold ExPTPR. 
       (*we need to split up F1 into the prelude and original part *)
-      apply relpower_comb_split in F1 as (x0 & H1 & H2 & H3). 
+      apply (@relpower_comb_split Sigma p t initCond l A0 Sigma' p' preludeInitialPred t' A1p A2p initialString initialString_validPreludeInitial) in F1 as (x0 & H1 & H2 & H3). 
       specialize (A1 H1) as (x & ->). exists x. split; [ | split]. 
       + apply relpower_valid_length_inv in H2. rewrite map_length in H2. 
-        apply relpower_valid_length_inv in H1. rewrite !map_length in H1. lia. 
+        apply relpower_valid_length_inv in H1. rewrite !map_length in H1. rewrite <- A5, H1. easy. 
       + apply A4 in H1. destruct H1 as (? & H1 & H4). apply Prelim.map_inj in H1; [subst; apply H4 | ]. 
         unfold injective. intros. congruence. 
       + unfold PTPRLang. split. 
@@ -276,7 +374,7 @@ Section fixPTPRInstance.
           unfold PTPR_wellformed. cbn. 
           apply relpower_valid_length_inv in H1. rewrite !map_length in H1. lia. }
         cbn. destruct H3 as (sf' & ->). exists sf'. split. 
-        * clear F2 A2 A3 A4. apply liftOrig_relpower_p, H2. 
+        * clear F2 A2 A3 A4. eapply liftOrig_relpower_p, H2. 
           apply relpower_valid_length_inv in H1.  rewrite !map_length in H1. lia.
         * clear A0 A2 A3 A4 A5 H1 H2. unfold satFinal in *. 
           destruct F2 as (subs & H1 & H2). apply in_map_iff in H1 as (subs' & <- & H1).
@@ -287,4 +385,4 @@ Section fixPTPRInstance.
           exists b1', b2'. enough (subs' = b') by (subst; reflexivity). 
           apply Prelim.map_inj in H2; [apply H2 | unfold injective; congruence].  
   Qed. 
-End fixPTPRInstance. 
+End fixPrelude. 
